cakeSemantics/CakeAST.v
@@ -4,8 +4,8 @@ Require Import BinNums.
 Require Import String.
 Require Import ZArith.BinInt.
 
-Require Import CakeSem.Namespace.
 Require Import CakeSem.Utils.
+Require Import CakeSem.Namespace.
 
 (* Literal constants *)
 Inductive lit : Type :=
@@ -398,4 +398,130 @@ Definition dec_ind (P : dec -> Prop) := dec_rect P.
 
 
 (** End induction principle *)
+(*-------------------------------------------------------------------*)
+
+(** Decidable Equality for terms, patterns, and expressions *)
+(*-------------------------------------------------------------------*)
+
+Theorem lit_eq_dec (l l' : lit) : {l = l'} + {l <> l'}.
+  decide equality; auto with DecidableEquality.  Defined.
+Hint Resolve lit_eq_dec : DecidableEquality.
+
+Theorem opn_eq_dec (o o' : opn) : {o = o'} + {o <> o'}.
+ decide equality. Defined.
+Hint Resolve opn_eq_dec : DecidableEquality.
+
+Theorem opb_eq_dec (o o' : opn) : {o = o'} + {o <> o'}.
+  decide equality.
+Defined.
+Hint Resolve opb_eq_dec : DecidableEquality.
+
+Theorem opw_eq_dec (o o' : opn) : {o = o'} + {o <> o'}.
+  decide equality.
+Defined.
+Hint Resolve opw_eq_dec : DecidableEquality.
+
+Theorem shift_eq_dec (o o' : opn) : {o = o'} + {o <> o'}.
+  decide equality.
+Defined.
+Hint Resolve shift_eq_dec : DecidableEquality.
+
+Theorem op_eq_dec : forall (o0 o1 : op), {o0 = o1} + {o0 <> o1}.
+Proof. repeat decide equality.  Defined.
+Hint Resolve op_eq_dec : DecidableEquality.
+
+Theorem lop_eq_dec : forall (l0 l1 : lop), {l0 = l1} + {l0 <> l1}.
+Proof. decide equality.  Defined.
+Hint Resolve lop_eq_dec : DecidableEquality.
+
+Theorem ast_t_eq_dec : forall (a1 a2 : ast_t), {a1 = a2} + {a1 <> a2}.
+Proof.
+  decide equality; auto with DecidableEquality; try (apply ident_eq_dec; apply string_dec);
+  generalize dependent l0;
+  induction H; destruct l0;
+    try (left; reflexivity);
+    try (right; discriminate);
+    try (destruct (p a);
+         destruct (IHForall'' l0);
+         try (inversion e0);
+         try (right; intro con; injection con; contradiction);
+         rewrite e; left; reflexivity).
+Defined.
+Hint Resolve ast_t_eq_dec : DecidableEquality.
+
+Theorem constr_id_eq_dec : forall (c0 c1 : constr_id), {c0 = c1} + {c0 <> c1}.
+Proof.
+  decide equality. auto with DecidableEquality.  Defined.
+Hint Resolve constr_id_eq_dec : DecidableEquality.
+
+Theorem pat_eq_dec : forall (p0 p1 : pat), {p0 = p1} + {p0 <> p1}.
+Proof. decide equality; auto with DecidableEquality.
+       generalize dependent l0.
+         induction l; destruct l0; try (left; reflexivity); try (right; discriminate).
+       inv X.
+       destruct (X0 p); subst.
+       destruct (IHl X1 l0); subst.
+       - left; reflexivity.
+       - right; intro con; inversion con; auto.
+       - right; intro con; inversion con; auto.
+Defined.
+Hint Resolve pat_eq_dec : DecidableEquality.
+
+Theorem typeDef_eq_dec : forall (t0 t1 : typeDef), {t0 = t1} + {t0 <> t1}.
+Proof. decide equality. decide equality.
+       apply list_eq_dec; decide equality; auto with DecidableEquality.
+       auto with DecidableEquality.  Defined.
+Hint Resolve typeDef_eq_dec : DecidableEquality.
+
+Theorem locs_eq_dec : forall (l0 l1 : locs), {l0 = l1} + {l0 <> l1}.
+Proof.
+  decide equality.
+  auto with DecidableEquality.
+Defined.
+Hint Resolve locs_eq_dec : DecidableEquality.
+
+Theorem exp_eq_dec : forall (e0 e1 : exp), {e0 = e1} + {e0 <> e1}.
+Proof.
+  decide equality; auto with DecidableEquality;
+    try (decide equality; try (apply ident_eq_dec); apply string_dec); generalize dependent l0.
+
+  induction X0; destruct l0.
+  - left; reflexivity.
+  - right; discriminate.
+  - right; discriminate.
+  - destruct x; destruct p0; simpl in *.
+    destruct (pat_eq_dec p1 p0); destruct (p e4); destruct (IHX0 l0); subst;
+      try (right; injection; auto); (left; reflexivity).
+  - induction X; destruct l0; try (left; reflexivity); try (right; discriminate).
+    destruct (p e); destruct (IHX l0); subst; try (right; injection; auto); left; reflexivity.
+  - induction X; destruct l0; try (left; reflexivity); try (right; discriminate).
+    destruct (p e); destruct (IHX l0); subst; try (right; injection; auto); left; reflexivity.
+  - induction X0; destruct l0; try (left; reflexivity); try (right; discriminate).
+    destruct x; destruct p0; simpl in *.
+    destruct (p e4); destruct (pat_eq_dec p1 p0); destruct (IHX0 l0); subst;
+      try (right; injection; auto); left; reflexivity.
+  - induction X; destruct l0; try (left; reflexivity); try (right; discriminate).
+    destruct x as [x' xe]; destruct x' as [xv0 xv1];
+      destruct p0 as [p0' p0e]; destruct p0' as [p0v0 p0v1]; simpl in *.
+    destruct (p p0e); destruct (string_dec xv0 p0v0); destruct (string_dec xv1 p0v1); destruct (IHX l0); subst;
+      try (right; injection; auto); left; reflexivity.
+Defined.
+Hint Resolve exp_eq_dec : DecidableEquality.
+
+Theorem dec_eq_dec : forall (d0 d1 : dec), {d0 = d1} + {d0 <> d1}.
+Proof.
+  decide equality; try (auto with DecidableEquality).
+  - generalize dependent l0. induction X; destruct l0; try (left; reflexivity); try (right; discriminate).
+    destruct (p d); destruct (IHX l0); subst; try (right; injection; auto); left; reflexivity.
+  - generalize dependent l2. induction X0; destruct l2; try (left; reflexivity); try (right; discriminate).
+    destruct (p d); destruct (IHX0 l2); subst; try (right; injection; auto); left; reflexivity.
+  - generalize dependent l; induction X.
+    + destruct l.
+      * left; reflexivity.
+      * right; discriminate.
+    + destruct l0.
+      * right; discriminate.
+      * destruct (p d); destruct (IHX l0); subst; try (right; injection; auto); left; reflexivity.
+Defined.
+Hint Resolve dec_eq_dec : DecidableEquality.
 (*-------------------------------------------------------------------*)
