cakeSemantics/Evaluate.v
@@ -1,40 +1,37 @@
-(** This file is DEPRECATED and probably does not compile *)
-
-
-
-
-
-
-
-From TLC Require Import LibLogic LibReflect.
-Require Import CakeSem.CakeAST.
-Require Import CakeSem.Namespace.
-Require Import CakeSem.SemanticPrimitives.
-Require Import CakeSem.ffi.FFI.
 Require Import CakeSem.Utils.
+Require Import CakeSem.ffi.FFI.
+Require Import CakeSem.Namespace.
+Require Import CakeSem.CakeAST.
+Require Import CakeSem.FreeVars.
+Require Import CakeSem.SemanticsAux.
 
 Require Import PeanoNat.
 Require Import List.
+Require Import ListDec.
+Require Import Ascii.
+Import Peano_dec.
+Import ZArith_dec.
 Import ListNotations.
 
 (* ---------------------------------------------------------------------- *)
-(** ** Store assign *)
+(** ** Helper functions *)
+Definition ident_string_dec := ident_eq_dec _ _ string_dec string_dec.
 
+(* ---------------------------------------------------------------------- *)
+(** ** Store assign *)
 Fixpoint store_assign {A : Type} (n : nat) (v : store_v A) (st : store A) : option (store A) :=
   match List.nth_error st n with
   | Some v' => if store_v_same_type v' v
-                 then Some (List.update n v st)
-                 else None
+              then Some (update n v st)
+              else None
   | _ => None
   end.
-
-
 
 (* ---------------------------------------------------------------------- *)
 (** ** Constructor comparison *)
 
 Definition same_ctor (s1 s2 : stamp) : bool :=
-  If s1 = s2 then true else false.
+  if stamp_eq_dec s1 s2 then true else false.
 
 
 (* ---------------------------------------------------------------------- *)
@@ -43,7 +40,7 @@ Definition same_ctor (s1 s2 : stamp) : bool :=
 Definition build_conv (envC : env_ctor) (cn : constr_id) (vs : list val) : option val :=
   match cn with
   | None => Some (Conv None vs)
-  | Some id => match nsLookup id envC with
+  | Some id => match nsLookupd id envC ident_string_dec with
               | None => None
               | Some (len,stamp) => Some (Conv (Some stamp) vs)
               end
@@ -84,21 +81,18 @@ Fixpoint pmatch (envC : env_ctor) (s : store val) (p : pat) (v : val)
   match p, v with
   | Pany, v' => Match env
   | Pvar x, v' => Match ((x,v')::env)
-  | Plit l, Litv l' => If l = l'
+  | Plit l, Litv l' => if lit_eq_dec l l'
                       then Match env
                       else if lit_same_type l l'
                            then No_match
                            else Match_type_error
   | Pcon (Some n) ps, Conv (Some stamp') vs =>
-    match  nsLookup n envC with
-    | Some (l, stamp) => If   istrue (same_type stamp stamp') (* LATER: same_type could be in Prop? *)
-                           /\ (length ps = l)
-                        then if same_ctor stamp stamp'
-                             then If (length ps = l) (* TODO: suspicious redundant test *)
-                                  then pmatch_list envC s ps vs env
-                                  else Match_type_error
-                             else No_match
-                        else Match_type_error
+    match  nsLookupd n envC ident_string_dec with
+    | Some (l, stamp) =>  if same_ctor stamp stamp'
+                         then if eq_nat_dec (length ps) l (* TODO: suspicious redundant test *)
+                              then pmatch_list envC s ps vs env
+                              else Match_type_error
+                         else No_match
     | _ => Match_type_error
     end
   | Pcon None ps, Conv None vs => pmatch_list envC s ps vs env
@@ -126,9 +120,9 @@ Definition do_con_check (cenv : env_ctor)
            (l : nat) : bool := (* LATER: switch to Prop *)
   match n_opt with
   | None => true
-  | Some n => match nsLookup n cenv with
+  | Some n => match nsLookupd n cenv ident_string_dec with
              | None => false
-             | Some (l',_) => If l = l' then true else false
+             | Some (l',_) => if Nat.eqb l l' then true else false
              end
   end.
 
@@ -137,8 +131,9 @@ Definition do_con_check (cenv : env_ctor)
 (** ** Equality test *)
 
 Inductive eq_result : Type :=
-  | Eq_val : bool -> eq_result
-  | Eq_type_error.
+| Eq_val : bool -> eq_result
+| Eq_type_error.
+Import Sumbool.
 
 (* Here we can probably start Prop-ertizing *) (* LATER: ask about it *)
 Fixpoint do_eq (e1 e2 : val) : eq_result :=
@@ -156,15 +151,15 @@ Fixpoint do_eq (e1 e2 : val) : eq_result :=
   in
   match e1, e2 with
   | Litv l1, Litv l2 => if lit_same_type l1 l2
-                       then Eq_val (If (l1 = l2) then true else false)
+                       then Eq_val (proj1_sig (bool_of_sumbool (lit_eq_dec l1 l2)))
                        else Eq_type_error
-  | Loc l1, Loc l2 => Eq_val (If (l1 = l2) then true else false)
-  | Conv cn1 vs1, Conv cn2 vs2 => If cn1 = cn2 /\ length vs1 = length vs2
+  | Loc l1, Loc l2 => Eq_val (Nat.eqb l1 l2)
+  | Conv cn1 vs1, Conv cn2 vs2 => if sumbool_and _ _ _ _ (option_eq_dec stamp stamp_eq_dec cn1 cn2) (eq_nat_dec (length vs1) (length vs2))
                                  then do_eq_list vs1 vs2
                                  else if ctor_same_type cn1 cn2
                                       then Eq_val false
                                       else Eq_type_error
-  | Vectorv vs1, Vectorv vs2 => If (length vs1 = length vs2)
+  | Vectorv vs1, Vectorv vs2 => if eq_nat_dec (length vs1) (length vs2)
                                then do_eq_list vs1 vs2
                                else Eq_val false
   | Closure _ _ _, Closure _ _ _ => Eq_val true
@@ -186,7 +181,7 @@ Fixpoint do_opapp (vs : list val) : option (sem_env val * exp) :=
   | (Closure env n e)::v::[] =>
     Some (update_sev env (nsBind n v (sev env)), e)
   | (Recclosure env funs n)::v::[] =>
-    if NoDup_dec String.string_dec
+    if NoDuplicates_dec String.string_dec
                  (List.map (fun p => match p with (f,x,e) => f end) funs)
     then match find_recfun n funs with
          | Some (n,e) =>
@@ -203,22 +198,22 @@ Fixpoint do_opapp (vs : list val) : option (sem_env val * exp) :=
 
 Definition store_ffi (ffi' : Type) (V : Type) := (store V * ffi_state ffi')%type.
 
+Definition natFromInteger (size : nat) :=
+      let fix helper (n' : nat ) (z : Z) : nat :=
+          match n' with
+          | O => O
+          | S n'' =>
+            (2 ^ n' * (Z.to_nat (Zdigits.bit_value
+                                            (Z.testbit (Z.of_nat n'') z)))
+                          + (helper n'' z))
+          end
+      in helper size.
+
+Definition word8FromInteger (i : Z) : word 8 := nat_to_word 8 (natFromInteger 8 i)%nat .
+Definition word64FromInteger (i : Z) : word 64 :=  nat_to_word 64 (natFromInteger 64%nat i).
+
 Fixpoint do_app (ffi' : Type) (st : store_ffi ffi' val) (o : op) (vs : list val)
   : option (store_ffi ffi' val * result val val) :=
-  (* LATER: take out as separate functions the next three defs *)
-  let natFromInteger  :=
-      (fun n : nat => let fix helper (n' : nat ) (z : Z) : nat :=
-                     match n' with
-                     | O => O
-                     | S n'' =>
-                       2 ^ n' * (Z.to_nat (Zdigits.bit_value
-                                            (Z.testbit (Z.of_nat n'') z)))
-                           + (helper n'' z)
-                     end
-                 in helper n)
-  in
-  let word8FromInteger  := fun i : Z => nat_to_word 8 (natFromInteger 8 i)%nat  in
-  let word64FromInteger := fun i : Z => nat_to_word 64 (natFromInteger 64%nat i) in
   match st with
     (s, t) =>
     match o, vs with
@@ -229,7 +224,7 @@ Fixpoint do_app (ffi' : Type) (st : store_ffi ffi' val) (o : op) (vs : list val)
       | _, _ => None
       end
     | Opn o', [Litv (IntLit n1); Litv (IntLit n2)] =>
-      If n2 = 0 /\ (o' = Divide \/ o' = Modulo)
+      if sumbool_and _ _ _ _ (Z.eq_dec n2 0) (sumbool_or _ _ _ _ (opn_eq_dec o' Divide) (opn_eq_dec o' Modulo))
         then Some ((s,t), Rerr (Rraise div_exn_v))
         else Some ((s,t), Rval (Litv (IntLit (opn_lookup o' n1 n2))))
     | Opb o', [Litv (IntLit n1); Litv (IntLit n2)] =>
@@ -267,7 +262,7 @@ Fixpoint do_app (ffi' : Type) (st : store_ffi ffi' val) (o : op) (vs : list val)
       | _ => None
       end
     | Aw8alloc, [Litv (IntLit n); Litv (Word8Lit w)] =>
-      If (n < 0)%Z then
+      if (Z_lt_dec n 0)%Z then
         Some ((s,t), Rerr (Rraise sub_exn_v))
       else
         let (s',lnum) := store_alloc (W8array (List.repeat w (Z.to_nat n))) s
@@ -275,7 +270,7 @@ Fixpoint do_app (ffi' : Type) (st : store_ffi ffi' val) (o : op) (vs : list val)
     | Aw8sub, [Loc lnum; Litv (IntLit i)] =>
       match store_lookup lnum s with
       | Some (W8array ws) =>
-        If (i < 0)%Z
+        if (Z_lt_dec i 0)%Z
         then Some ((s,t), Rerr (Rraise sub_exn_v))
         else
           let n := Z.to_nat i in
@@ -287,17 +282,17 @@ Fixpoint do_app (ffi' : Type) (st : store_ffi ffi' val) (o : op) (vs : list val)
       end
     | Aw8length, [Loc n] =>
       match store_lookup n s with
-      | Some (W8array ws) => Some ((s,t), Rval (Litv (IntLit (Zlength ws))))
+      | Some (W8array ws) => Some ((s,t), Rval (Litv (IntLit (ZArith.Zcomplements.Zlength ws))))
       | _ => None
       end
     | Aw8update, [Loc lnum; Litv (IntLit i); Litv (Word8Lit w)] =>
       match store_lookup lnum s with
       | Some (W8array ws) =>
-        If (i < 0)%Z then
+        if (Z_lt_dec i 0)%Z then
           Some ((s,t), Rerr (Rraise sub_exn_v))
         else
           let n := Z.to_nat i in
-          if leb (List.length ws) n then
+          if Nat.leb (List.length ws) n then
             Some ((s,t), Rerr (Rraise sub_exn_v))
           else
             match store_assign lnum (W8array (update n w ws)) s with
@@ -363,7 +358,7 @@ Fixpoint do_app (ffi' : Type) (st : store_ffi ffi' val) (o : op) (vs : list val)
     | Ord, [Litv (CharLit c)] =>
       Some ((s,t), Rval (Litv (IntLit (Z.of_nat (nat_of_ascii c)))))
     | Chr, [Litv (IntLit i)] =>
-      Some ((s,t), If (i < 0)%Z \/ (i > 255)%Z
+      Some ((s,t), if sumbool_and _ _ _ _ (Z_lt_dec i 0)%Z (Z_lt_dec 255 i)%Z
                    then Rerr (Rraise chr_exn_v)
                    else Rval (Litv (CharLit (ascii_of_nat (Z.to_nat i)))))
     | Chopb op, [Litv (CharLit c1); Litv (CharLit c2)] =>
@@ -375,7 +370,7 @@ Fixpoint do_app (ffi' : Type) (st : store_ffi ffi' val) (o : op) (vs : list val)
       | None => None
       end
     | Strsub, [Litv (StrLit str); Litv (IntLit i)] =>
-      If (i < 0)%Z then
+      if (Z_lt_dec i 0)%Z then
         Some ((s,t), Rerr (Rraise sub_exn_v))
       else
         let n := Z.to_nat i in
@@ -401,7 +396,7 @@ Fixpoint do_app (ffi' : Type) (st : store_ffi ffi' val) (o : op) (vs : list val)
       | None    => None
       end
     | VSub, [Vectorv vs; Litv (IntLit i)] =>
-      If (i < 0)%Z
+      if (Z_lt_dec i 0)%Z
       then Some ((s,t), Rerr (Rraise sub_exn_v))
       else
         let n := Z.to_nat i in
@@ -412,7 +407,7 @@ Fixpoint do_app (ffi' : Type) (st : store_ffi ffi' val) (o : op) (vs : list val)
     | Vlength, [Vectorv vs] =>
       Some ((s,t), Rval (Litv (IntLit (Z.of_nat (List.length  vs)))))
     | Aalloc, [Litv (IntLit n); v] =>
-      If (n < 0)%Z
+      if (Z_lt_dec n 0)%Z
       then Some ((s,t), Rerr (Rraise sub_exn_v))
       else
         let (s',lnum) := store_alloc (Varray (List.repeat v (Z.to_nat n))) s
@@ -423,7 +418,7 @@ Fixpoint do_app (ffi' : Type) (st : store_ffi ffi' val) (o : op) (vs : list val)
     | Asub, [Loc lnum; Litv (IntLit i)] =>
       match store_lookup lnum s with
       | Some (Varray vs) =>
-        If (i < 0)%Z then
+        if (Z_lt_dec i 0)%Z then
           Some ((s,t), Rerr (Rraise sub_exn_v))
         else
           let n := Z.to_nat i in
@@ -442,11 +437,11 @@ Fixpoint do_app (ffi' : Type) (st : store_ffi ffi' val) (o : op) (vs : list val)
     | Aupdate, [Loc lnum; Litv (IntLit i); v] =>
       match store_lookup lnum s with
       | Some (Varray vs') =>
-        If (i < 0)%Z then (* LATER: use a wrapper function for this kind of test *)
+        if (Z_lt_dec i 0)%Z then (* LATER: use a wrapper function for this kind of test *)
           Some ((s,t), Rerr (Rraise sub_exn_v))
         else
           let n := Z.to_nat i in
-          if leb (List.length vs') n
+          if Nat.leb (List.length vs') n
           then Some ((s,t), Rerr (Rraise sub_exn_v))
           else
             match store_assign lnum (Varray (update n v vs')) s with
@@ -482,46 +477,46 @@ Inductive exp_or_val : Type :=
 
 Definition do_log (op : lop) (v : val) (e : exp) : option exp_or_val :=
   match op with (* LATER: would be more idiomatic to write "If v = Boolv true" *)
-  | And => If (Boolv true) = v
+  | And => if val_eq_dec (Boolv true) v
           then Some (Exp e)
-          else If (Boolv false) = v
+          else if val_eq_dec (Boolv false) v
                then Some (Val v)
                else None
-  | Or => If (Boolv true) = v
+
+  | Or => if val_eq_dec (Boolv true) v
           then Some (Val v)
-          else If (Boolv false) = v
+          else if val_eq_dec (Boolv false) v
                then Some (Exp e)
                else None
   end.
 
 Definition do_if (v : val) (e1 e2 : exp) : option exp :=
-  If Boolv true = v
+  if val_eq_dec (Boolv true) v
     then Some e1
-    else If Boolv false = v
+    else if val_eq_dec (Boolv false) v
          then Some e2
          else None.
 
-
 (* ---------------------------------------------------------------------- *)
 
-Definition fix_clock {ffi' : Type} {res error : Type} (s : state ffi')
-           (p : state ffi' * result res error) : state ffi' * result res error :=
-  match p with (s', r) =>
-               ({| clock  := If clock s' <= clock s
-                           then clock s' else clock s;
-                   refs := refs s';
-                   ffi := ffi s';
-                   next_type_stamp := next_type_stamp s';
-                   next_exn_stamp := next_exn_stamp s' |}
-                , r)
-  end.
+(* Definition fix_clock {ffi' : Type} {res error : Type} (s : state ffi') *)
+(*            (p : state ffi' * result res error) : state ffi' * result res error := *)
+(*   match p with (s', r) => *)
+(*                ({| clock  := If clock s' <= clock s *)
+(*                            then clock s' else clock s; *)
+(*                    refs := refs s'; *)
+(*                    ffi := ffi s'; *)
+(*                    next_type_stamp := next_type_stamp s'; *)
+(*                    next_exn_stamp := next_exn_stamp s' |} *)
+(*                 , r) *)
+(*   end. *)
 
-Definition dec_clock {ffi' : Type} (s : state ffi') : state ffi' :=
-  {| clock := clock s - 1;
-     refs := refs s;
-     ffi := ffi s;
-     next_type_stamp := next_type_stamp s;
-     next_exn_stamp := next_exn_stamp s |}.
+(* Definition dec_clock {ffi' : Type} (s : state ffi') : state ffi' := *)
+(*   {| clock := clock s - 1; *)
+(*      refs := refs s; *)
+(*      ffi := ffi s; *)
+(*      next_type_stamp := next_type_stamp s; *)
+(*      next_exn_stamp := next_exn_stamp s |}. *)
 
 Definition list_result {A B : Type} (res : result A B) : result (list A) B :=
   match res with
@@ -529,122 +524,334 @@ Definition list_result {A B : Type} (res : result A B) : result (list A) B :=
   | Rerr e => Rerr e
   end.
 
-Definition v : Type := val. (* TODO: why? *)
 
-(* LATER: fix decreasing measure, e.g. using TLC's LibFix, or fuel argument *)
+Fixpoint evaluate (fuel : nat) {ffi' : Type} (st : state ffi') (env : sem_env val)
+         (es : list exp) : state ffi' * result (list val) val :=
+  match fuel with
+  | O => (st, Rerr (Rabort Rtimeout_error))
+  | S fuel' =>
+    let fix evaluate_match (st : state ffi') (env : sem_env val) (v' : val)
+            (pes : list (pat * exp)) (err_v : val) : state ffi' * result (list val) val :=
+        match pes with
+        | [] => (st, Rerr (Rraise err_v))
+        | (p,e)::pes' => if NoDuplicates_dec string_dec (pat_bindings p)
+                       then match pmatch (sec env) (refs st) p v' [] with
+                            | Match env_v' => evaluate fuel' st {| sev := nsAppend (alist_to_ns env_v') (sev env);
+                                                                  sec := (sec env) |} [e]
+                            | No_match => evaluate_match st env v' pes' err_v
+                            | Match_type_error => (st, Rerr (Rabort Rtype_error))
+                            end
+                       else (st, Rerr (Rabort Rtype_error))
+        end
+    in
 
-Fixpoint evaluate {ffi' : Type} (st : state ffi') (env : sem_env v)
-         (es : list exp) : state ffi' * result (list v) v :=
-
-  let fix evaluate_match (st : state ffi') (env : sem_env v) (v' : v)
-          (pes : list (pat * exp)) (err_v : v) : state ffi' * result (list v) v :=
-      match pes with
-      | [] => (st, Rerr (Rraise err_v))
-      | (p,e)::pes' => If LibList.noduplicates (pat_bindings p)
-                     then match pmatch (sec env) (refs st) p v' [] with
-                          | Match env_v' => evaluate st {| sev := nsAppend (alist_to_ns env_v') (sev env);
-                                                          sec := (sec env) |} [e]
-                          | No_match => evaluate_match st env v' pes' err_v
-                          | Match_type_error => (st, Rerr (Rabort Rtype_error))
-                          end
-                     else (st, Rerr (Rabort Rtype_error))
-      end
-  in
-
-  let fix evaluate_single_exp (st : state ffi') (env : sem_env v) (ex : exp)
-      : state ffi' * result (list v) v :=
-      match ex with
-      | ELit l => (st, Rval [Litv l])
-      | ERaise e => match evaluate_single_exp st env e with
-                  | (st', Rval (v'::vs')) => (st', Rerr (Rraise v'))
-                  | res => res
-                  end
-      | EHandle e pes => match (evaluate_single_exp st env e) with
-                       | (st', Rerr (Rraise v')) => evaluate_match st' env v' pes v'
-                       | res => res
-                       end
-      | ECon cn es' => if do_con_check (sec env) cn (length es')
-                     then match evaluate st env (rev es') with
-                          | (st', Rval vs) => match build_conv (sec env) cn (rev vs) with
-                                             | Some v' => (st', Rval [v'])
-                                             | None => (st', Rerr (Rabort Rtype_error))
-                                             end
-                          | res => res
-                          end
-                     else (st, Rerr (Rabort Rtype_error))
-      | EVar n => match nsLookup n (sev env) with
-                | Some v' => (st, Rval [v'])
-                | None => (st, Rerr (Rabort Rtype_error))
-                end
-      | EFun x e => (st, Rval [Closure env x e])
-
-      | EApp op es => match (evaluate st env (rev es)) with
-                     | (st', Rval vs) => If op = Opapp
-                                        then match do_opapp (rev vs) with
-                                             | Some (env', e) =>
-                                               if Peano_dec.eq_nat_dec (clock st') 0
-                                               then (st', Rerr (Rabort Rtimeout_error))
-                                               else evaluate (dec_clock st') env' [e]
-                                             | None => (st', Rerr (Rabort Rtype_error))
-                                             end
-                                        else match do_app _ (refs st', ffi st') op (rev vs) with
-                                             | Some ((refs, ffi), r) => ({| refs := refs;
-                                                                           ffi  := ffi;
-                                                                           clock := clock st';
-                                                                           next_type_stamp := next_type_stamp st' ;
-                                                                           next_exn_stamp := next_exn_stamp st'
-                                                                        |},
-                                                                        list_result r)
-                                             | None => (st', Rerr (Rabort Rtype_error))
-                                             end
+    let fix evaluate_single_exp (st : state ffi') (env : sem_env val) (ex : exp)
+        : state ffi' * result (list val) val :=
+        match ex with
+        | ELit l => (st, Rval [Litv l])
+        | ERaise e => match evaluate_single_exp st env e with
+                     | (st', Rval (v'::vs')) => (st', Rerr (Rraise v'))
                      | res => res
                      end
+        | EHandle e pes => match (evaluate_single_exp st env e) with
+                          | (st', Rerr (Rraise v')) => evaluate_match st' env v' pes v'
+                          | res => res
+                          end
+        | ECon cn es' => if do_con_check (sec env) cn (length es')
+                        then match evaluate fuel' st env (rev es') with
+                             | (st', Rval vs) => match build_conv (sec env) cn (rev vs) with
+                                                | Some v' => (st', Rval [v'])
+                                                | None => (st', Rerr (Rabort Rtype_error))
+                                                end
+                             | res => res
+                             end
+                        else (st, Rerr (Rabort Rtype_error))
+        | EVar n => match nsLookupd n (sev env) ident_string_dec with
+                   | Some v' => (st, Rval [v'])
+                   | None => (st, Rerr (Rabort Rtype_error))
+                   end
+        | EFun x e => (st, Rval [Closure env x e])
 
-      | ELog lop e1 e2 => match (evaluate st env [e1]) with
-                         | (st', Rval (v1::vs1)) => match do_log lop v1 e2 with
-                                                  | Some (Exp e) => evaluate st' env [e]
-                                                  | Some (Val v') => (st', Rval [v'])
+        | EApp op es => match (evaluate fuel' st env (rev es)) with
+                       | (st', Rval vs) => if op_eq_dec op Opapp
+                                          then match do_opapp (rev vs) with
+                                               | Some (env', e) =>
+                                                 if eq_nat_dec (clock st') 0
+                                                 then (st', Rerr (Rabort Rtimeout_error))
+                                                 else evaluate fuel' st' env' [e]
+                                               | None => (st', Rerr (Rabort Rtype_error))
+                                               end
+                                          else match do_app _ (refs st', ffi st') op (rev vs) with
+                                               | Some ((refs, ffi), r) => ({| refs := refs;
+                                                                             ffi  := ffi;
+                                                                             clock := clock st';
+                                                                             next_type_stamp := next_type_stamp st' ;
+                                                                             next_exn_stamp := next_exn_stamp st'
+                                                                          |},
+                                                                          list_result r)
+                                               | None => (st', Rerr (Rabort Rtype_error))
+                                               end
+                       | res => res
+                       end
+
+        | ELog lop e1 e2 => match (evaluate fuel' st env [e1]) with
+                           | (st', Rval (v1::vs1)) => match do_log lop v1 e2 with
+                                                    | Some (Exp e) => evaluate fuel' st' env [e]
+                                                    | Some (Val v') => (st', Rval [v'])
+                                                    | None => (st', Rerr (Rabort Rtype_error))
+                                                    end
+                           | res => res
+                           end
+
+        | EIf e1 e2 e3 => match (evaluate fuel' st env [e1]) with
+                         | (st', Rval (v'::vs')) => match do_if v' e2 e3 with
+                                                  | Some e => evaluate fuel' st' env [e]
                                                   | None => (st', Rerr (Rabort Rtype_error))
                                                   end
                          | res => res
                          end
 
-      | EIf e1 e2 e3 => match (evaluate st env [e1]) with
-                       | (st', Rval (v'::vs')) => match do_if v' e2 e3 with
-                                                | Some e => evaluate st' env [e]
-                                                | None => (st', Rerr (Rabort Rtype_error))
-                                                end
+        | EMat e pes => match (evaluate fuel' st env [e]) with
+                       | (st', Rval (v'::vs')) => evaluate_match st' env v' pes bind_exn_v
                        | res => res
                        end
 
-      | EMat e pes => match (evaluate st env [e]) with
-                     | (st', Rval (v'::vs')) => evaluate_match st' env v' pes bind_exn_v
-                     | res => res
-                     end
+        | ELet xo e1 e2 => match (evaluate fuel' st env [e1]) with
+                          | (st', Rval (v'::vs')) => evaluate fuel' st'
+                                                            {| sev := nsOptBind xo v' (sev env); sec := (sec env) |} [e2]
+                          | res => res
+                          end
 
-      | ELet xo e1 e2 => match (evaluate st env [e1]) with
-                        | (st', Rval (v'::vs')) => evaluate st'
-                                {| sev := nsOptBind xo v' (sev env); sec := (sec env) |} [e2]
-                        | res => res
-                        end
+        | ELetrec funs e =>  if NoDuplicates_dec (pair_eq_dec _ _ (pair_eq_dec _ _ string_dec string_dec) exp_eq_dec) funs
+                            then evaluate fuel' st {| sev := build_rec_env funs env (sev env); sec := (sec env) |} [e]
+                            else (st, Rerr (Rabort Rtype_error))
 
-      | ELetrec funs e => If LibList.noduplicates (map (fun trip => match trip with (x, y, z) => x end) funs)
-                         then evaluate st {| sev := build_rec_env funs env (sev env); sec := (sec env) |} [e]
-                         else (st, Rerr (Rabort Rtype_error))
+        | ETannot e t => evaluate fuel' st env [e]
+        | ELannot e l => evaluate fuel' st env [e]
+        end
+    in
 
-      | ETannot e t => evaluate st env [e]
-      | ELannot e l => evaluate st env [e]
-      end
-  in
-
-  match es with
-  | [] => (st, Rval [])
-  | e'::es' => match evaluate_single_exp st env e' with
-             | (st', Rval (v'::vs')) =>
-               match evaluate st' env es' with
-               | (st'', Rval vs'') => (st'', Rval (v'::vs''))
+    match es with
+    | [] => (st, Rval [])
+    | e'::es' => match evaluate_single_exp st env e' with
+               | (st', Rval (v'::vs')) =>
+                 match evaluate fuel' st' env es' with
+                 | (st'', Rval vs'') => (st'', Rval (v'::vs''))
+                 | res => res
+                 end
                | res => res
                end
-             | res => res
-             end
+    end
   end.
+
+Fixpoint evaluate_opt (fuel : nat) {ffi' : Type} (st : state ffi') (env : sem_env val)
+         (es : list exp) : state ffi' * result (list val) val :=
+  match fuel with
+  | O => (st, Rerr (Rabort Rtimeout_error))
+  | S fuel' =>
+    let fix evaluate_match (st : state ffi') (env : sem_env val) (v' : val)
+            (pes : list (pat * exp)) (err_v : val) : state ffi' * result (list val) val :=
+        match pes with
+        | [] => (st, Rerr (Rraise err_v))
+        | (p,e)::pes' => if NoDuplicates_dec string_dec (pat_bindings p)
+                       then match pmatch (sec env) (refs st) p v' [] with
+                            | Match env_v' => evaluate_opt fuel' st {| sev := nsAppend (alist_to_ns env_v') (sev env);
+                                                                  sec := (sec env) |} [e]
+                            | No_match => evaluate_match st env v' pes' err_v
+                            | Match_type_error => (st, Rerr (Rabort Rtype_error))
+                            end
+                       else (st, Rerr (Rabort Rtype_error))
+        end
+    in
+
+    let fix evaluate_single_exp (st : state ffi') (env : sem_env val) (ex : exp)
+        : state ffi' * result (list val) val :=
+        match ex with
+        | ELit l => (st, Rval [Litv l])
+        | ERaise e => match evaluate_single_exp st env e with
+                     | (st', Rval (v'::vs')) => (st', Rerr (Rraise v'))
+                     | res => res
+                     end
+        | EHandle e pes => match (evaluate_single_exp st env e) with
+                          | (st', Rerr (Rraise v')) => evaluate_match st' env v' pes v'
+                          | res => res
+                          end
+        | ECon cn es' => if do_con_check (sec env) cn (length es')
+                        then match evaluate_opt fuel' st env (rev es') with
+                             | (st', Rval vs) => match build_conv (sec env) cn (rev vs) with
+                                                | Some v' => (st', Rval [v'])
+                                                | None => (st', Rerr (Rabort Rtype_error))
+                                                end
+                             | res => res
+                             end
+                        else (st, Rerr (Rabort Rtype_error))
+        | EVar n => match nsLookupd n (sev env) ident_string_dec with
+                   | Some v' => (st, Rval [v'])
+                   | None => (st, Rerr (Rabort Rtype_error))
+                   end
+        | EFun x e => (st, Rval [Closure (optimize_sem_env env (free_vars e)) x e])
+
+        | EApp op es => match (evaluate_opt fuel' st env (rev es)) with
+                       | (st', Rval vs) => if op_eq_dec op Opapp
+                                          then match do_opapp (rev vs) with
+                                               | Some (env', e) =>
+                                                 if eq_nat_dec (clock st') 0
+                                                 then (st', Rerr (Rabort Rtimeout_error))
+                                                 else evaluate_opt fuel' st' env' [e]
+                                               | None => (st', Rerr (Rabort Rtype_error))
+                                               end
+                                          else match do_app _ (refs st', ffi st') op (rev vs) with
+                                               | Some ((refs, ffi), r) => ({| refs := refs;
+                                                                             ffi  := ffi;
+                                                                             clock := clock st';
+                                                                             next_type_stamp := next_type_stamp st' ;
+                                                                             next_exn_stamp := next_exn_stamp st'
+                                                                          |},
+                                                                          list_result r)
+                                               | None => (st', Rerr (Rabort Rtype_error))
+                                               end
+                       | res => res
+                       end
+
+        | ELog lop e1 e2 => match (evaluate_opt fuel' st env [e1]) with
+                           | (st', Rval (v1::vs1)) => match do_log lop v1 e2 with
+                                                    | Some (Exp e) => evaluate_opt fuel' st' env [e]
+                                                    | Some (Val v') => (st', Rval [v'])
+                                                    | None => (st', Rerr (Rabort Rtype_error))
+                                                    end
+                           | res => res
+                           end
+
+        | EIf e1 e2 e3 => match (evaluate_opt fuel' st env [e1]) with
+                         | (st', Rval (v'::vs')) => match do_if v' e2 e3 with
+                                                  | Some e => evaluate_opt fuel' st' env [e]
+                                                  | None => (st', Rerr (Rabort Rtype_error))
+                                                  end
+                         | res => res
+                         end
+
+        | EMat e pes => match (evaluate_opt fuel' st env [e]) with
+                       | (st', Rval (v'::vs')) => evaluate_match st' env v' pes bind_exn_v
+                       | res => res
+                       end
+
+        | ELet xo e1 e2 => match (evaluate_opt fuel' st env [e1]) with
+                          | (st', Rval (v'::vs')) => evaluate_opt fuel' st'
+                                                            {| sev := nsOptBind xo v' (sev env); sec := (sec env) |} [e2]
+                          | res => res
+                          end
+
+        | ELetrec funs e =>  if NoDuplicates_dec (pair_eq_dec _ _ (pair_eq_dec _ _ string_dec string_dec) exp_eq_dec) funs
+                            then evaluate_opt fuel' st {| sev := build_rec_env funs env (sev env); sec := (sec env) |} [e]
+                            else (st, Rerr (Rabort Rtype_error))
+
+        | ETannot e t => evaluate_opt fuel' st env [e]
+        | ELannot e l => evaluate_opt fuel' st env [e]
+        end
+    in
+
+    match es with
+    | [] => (st, Rval [])
+    | e'::es' => match evaluate_single_exp st env e' with
+               | (st', Rval (v'::vs')) =>
+                 match evaluate_opt fuel' st' env es' with
+                 | (st'', Rval vs'') => (st'', Rval (v'::vs''))
+                 | res => res
+                 end
+               | res => res
+               end
+    end
+  end.
+
+Fixpoint evaluate_decs {ffi' : Type} (fuel : nat) (st : state ffi') (env : sem_env val) (decl : list dec) :
+  (state ffi' * result (sem_env val) val) :=
+  match fuel with
+  | O => (st, Rerr (Rabort Rtimeout_error))
+  | S fuel' =>
+    match decl with
+    | [] => (st, Rval empty_sem_env)
+    | d1::d2::decl' => match evaluate_decs fuel' st env [d1] with
+                    | (st1, Rval env1) =>
+                      match evaluate_decs fuel' st (extend_dec_env env1 env) (d2::decl') with
+                      | (st2, r) => (st2, combine_dec_result env1 r)
+                      end
+                    | res => res
+                    end
+
+
+    | [Dlet locs p e] =>
+      if NoDuplicates_dec string_dec (pat_bindings p)
+      then match evaluate fuel st env [e] with
+           | (st', Rval v) =>
+             (st', match pmatch (sec env) (refs st') p (hd (Litv (StrLit "IF HERE THEN BAD")) v) [] with
+                   | Match new_vals => Rval {| sec := nsEmpty; sev := alist_to_ns new_vals |}
+                   | No_match => Rerr (Rraise bind_exn_v)
+                   | Match_type_error => Rerr (Rabort Rtype_error)
+                   end)
+           | (st', Rerr err) => (st', Rerr err)
+           end
+      else (st, Rerr (Rabort Rtype_error))
+
+    | [Dletrec locs funs] => (st,
+                             if NoDuplicates_dec string_dec (map (fun x => fst (fst x)) funs)
+                             then Rval {| sev := build_rec_env funs env nsEmpty; sec := nsEmpty |}
+                             else Rerr (Rabort Rtype_error))
+
+    | [Dtype locs tds] => if UniqueCtorsInDefs_dec tds
+                         then (state_update_next_type_stamp st (next_type_stamp st + List.length tds),
+                              Rval {| sev := nsEmpty; sec := build_tdefs (next_type_stamp st) tds |})
+                         else (st, Rerr (Rabort Rtype_error))
+  | [Dtabbrev locs tvs tn t] => (st, Rval {| sev := nsEmpty; sec := nsEmpty |})
+  | [Dexn locs cn ts] => (state_update_next_exn_stamp st (next_exn_stamp st + 1),
+                         Rval {| sev := nsEmpty;
+                                 sec := nsSing cn (List.length ts, ExnStamp (next_exn_stamp st)) |})
+  | [Dmod mn ds] => match evaluate_decs fuel' st env ds with
+                   | (st', r) => (st',
+                                 match r with
+                                 | Rval env' => Rval {| sev := nsLift mn (sev env');
+                                                       sec := nsLift mn (sec env') |}
+                                 | Rerr err => Rerr err
+                                 end)
+                   end
+  | [Dlocal lds ds] => match evaluate_decs fuel' st env lds with
+                      | (st1, Rval env1) =>
+                        evaluate_decs fuel' st1 (extend_dec_env env1 env) ds
+                      | res => res
+                      end
+    end
+  end.
+
+(* Trying to remove fuel from the evaluate_decs *)
+(* Fixpoint evaluate_decs {ffi' : Type} (fuel : nat) (st : state ffi') (env : sem_env val) (decl : list dec) : *)
+(*   (state ffi' * result (sem_env val) val) := *)
+(*   match decl with *)
+(*   | [] => (st, Rval empty_sem_env) *)
+(*   | d::decl' => *)
+(*     match d with *)
+(*     | Dlet locs p e => *)
+(*       if @NoDup_dec varN string_dec (pat_bindings p) *)
+(*       then match evaluate fuel st env [e] with *)
+(*            | (st', Rval v) => *)
+(*              (st', *)
+(*               match pmatch (sec env) (refs st') p *)
+(*                            (hd (Litv (StrLit "THIS IS BAD IF THIS VALUE IS RETURNED")) v) with *)
+(*               | Match new_vals => *)
+(*                 match evaluate_decs fuel st' (extend_dec_env (build_sem_env ns_empty new_vals) env) decl' with *)
+(*                 | (st'', Rerr err) *)
+(*               | No_match => Rerr (Rraise bind_exn_v) *)
+(*               | Match_type_eror => Rerr (Rabort Rtype_error) *)
+(*               end) *)
+(*            | (st', Rerr err) => (* FAKE *) (st, Rval empty_sem_env) *)
+(*            end *)
+(*       else (st, Rerr (Rabort Rtype_error)) *)
+
+
+
+(*     | Dletrec locs funs => (* FAKE *) (st, Rval empty_sem_env) *)
+(*     | Dtype locs tds => (* FAKE *) (st, Rval empty_sem_env) *)
+(*     | Dtabbrev locs tvs tn t => (* FAKE *) (st, Rval empty_sem_env) *)
+(*     | Dexn locs cn ts => (* FAKE *) (st, Rval empty_sem_env) *)
+(*     | Dmod mn ds => (* FAKE *) (st, Rval empty_sem_env) *)
+(*     | Dlocal lds ds => (* FAKE *) (st, Rval empty_sem_env) *)
+(*     end *)
+(*   end. *)
