cakeSemantics/Namespace.v
@@ -4,6 +4,7 @@ Import ListNotations.
 Require Import Structures.Equalities.
 Require Import Classes.EquivDec.
 Require Import Program.Utils.
+Require Import CakeSem.Utils.
 
 Definition alist (X Y : Type) := list (X * Y).
 
@@ -55,10 +56,6 @@ Fixpoint get_modded_namespace {M N V : Type} (m : M) (ns : namespace M N V) : na
   end.
 
 Definition nsLookup {M N V : Type} (id : ident M N) (ns : namespace M N V) : option V := lookup id ns.
-  (* match id with *)
-  (* | Short n => lookup id ns *)
-  (* | Long m id' => nsLookup id' (get_modded_namespace m ns) *)
-  (* end. *)
 
 (* LATER: use LibList.filter *)
 
@@ -121,14 +118,6 @@ Definition eAll2 {M N V1 V2 : Type} (rel : ident M N -> V1 -> V2 -> Prop)
   (ns1 : namespace M N V1) (ns2 : namespace M N V2) : Prop :=
   nsSub rel ns1 ns2 /\ nsSub (fun x y z => rel x z y) ns2 ns1.
 
-(* LATER: fix this *)
-(* Need to construct a set of id's that are bound. *)
-
-(* Definition nsDom {M N V : Type} `{Eq M} `{Eq N} `{Eq V} SetType V (ns : namespace M N V) : set (Id M N) := *)
-
- (*  nsLookup ns id = Just v *)
- (* { n | forall (v IN universal) (n IN universal) | nsLookup env n = Just v } *)
-
 Definition extractIds {M N V : Type} (ns : namespace M N V) : list (ident M N) :=
   map fst ns.
 
@@ -144,13 +133,165 @@ Fixpoint extractMods {M N V : Type} (ns : namespace M N V) : list (list M) :=
   | (id,_)::ns' => get_ids id :: extractMods ns'
   end.
 
-(* Definition nsDomMod : {M N V : Type} `{Eq M} `{Eq N} `{Eq V} SetType V (ns : namespace M N V) : set (list M) := *)
-
-(* let nsDomMod env = { n | forall (v IN universal) (n IN universal) | nsLookupMod env n = Just v } *)
-
 Fixpoint nsMap {M N V W : Type} (f : V -> W)
          (ns : namespace M N V) : namespace M N W :=
   map (fun '(i1,i2) => (i1, f i2)) ns.
 
-(* LATER: use List.map
-   LATER: avoid fst/snd where possible *)
+(* Namespace functions using a sumbool type for equality tests *)
+Fixpoint lookupd {X Y : Type} (x : X) (l : alist X Y) (f : forall (x1 x2 : X), {x1 = x2} + {x1 <> x2}): option Y :=
+  match l with
+  | [] => None
+  | (x',y) :: l' => if f x x' then Some y else lookupd x l' f
+  end.
+
+Fixpoint get_modded_namespaced {M N V : Type} (m : M) (ns : namespace M N V)
+         (f : forall (x1 x2 : M), {x1 = x2} + {x1 <> x2}) : namespace M N V :=
+  match ns with
+  | [] => []
+  | (i,v) :: ns' => match i with
+                    | Short _ => get_modded_namespaced m ns' f
+                    | Long m' i' => if f m m'
+                                   then (i',v) :: (get_modded_namespaced m ns' f)
+                                   else get_modded_namespaced m ns' f
+                  end
+  end.
+
+Definition nsLookupd {M N V : Type} (id : ident M N) (ns : namespace M N V)
+           (f : forall (x1 x2 : ident M N), {x1 = x2} + {x1 <> x2}) : option V := lookupd id ns f.
+
+Fixpoint nsLookupModd {M N V : Type} (ns : namespace M N V) (xs : list M) (f_dec : forall m1 m2 : M, {m1 = m2} + {m1 <> m2}) : option (namespace M N V) :=
+  match xs, ns with
+  | _, [] => None
+  | [], ns => Some ns
+  | m :: ms, ns => nsLookupModd (filter (fun '(i1,i2) => match i1 with
+                                            | Short n    => false
+                                            | Long  m' n => if f_dec m m' then true else false
+                                            end)
+                                     ns)
+                             ms
+                             f_dec
+  end.
+
+(* Namespace Theorems *)
+Section NamespaceDec.
+  Variable M : Type.
+  Variable N : Type.
+  Variable V : Type.
+  Hypothesis HM : forall (m0 m1 : M), {m0 = m1} + {m0 <> m1}.
+  Hypothesis HN : forall (n0 n1 : N), {n0 = n1} + {n0 <> n1}.
+  Hypothesis HV : forall (v0 v1 : V), {v0 = v1} + {v0 <> v1}.
+
+  Theorem ident_eq_dec : forall (i0 i1 : ident M N),
+      {i0 = i1} + {i0 <> i1}.
+  Proof. decide equality.  Defined.
+
+  Theorem namespace_eq_dec : forall (n0 n1 : namespace M N V), {n0 = n1} + {n0 <> n1}.
+  Proof. decide equality. decide equality. apply ident_eq_dec. Defined.
+End NamespaceDec.
+Hint Resolve namespace_eq_dec : DecidableEquality.
+Hint Resolve ident_eq_dec : DecidableEquality.
+
+Section LookupTheory.
+  Variable N : Type.
+  Variable V : Type.
+
+  Lemma lookup_cover : forall (n : N) (ns ns' : alist N V) (v : V),
+      lookup n ns = Some v ->
+      lookup n (ns ++ ns') = lookup n ns.
+  Proof.
+    intros n ns ns' v.
+    generalize dependent ns'.
+    induction ns; intros ns' H.
+    - inversion H.
+    - destruct a. inversion H; subst; clear H.
+      assert ({n = n0} + {n <> n0}) by apply (classicT (n = n0)).
+      destruct H; simpl.
+      + rewrite e. rewrite 2 If_l; reflexivity.
+      + rewrite 2 If_r in *; try (assumption). apply IHns. assumption.
+  Qed.
+
+  Lemma lookup_drop : forall (id : N) (ns ns' : alist N V),
+      lookup id ns = None ->
+      lookup id (ns ++ ns') = lookup id ns'.
+  Proof.
+    intros id ns.
+    induction ns; intros ns' H.
+    - reflexivity.
+    - destruct a; simpl in *.
+      assert ({id = n} + {id <> n}) as loem by apply (classicT (id = n)).
+      destruct loem.
+      + rewrite <- e in *. rewrite If_l in H; try (reflexivity). inversion H.
+      + rewrite If_r in *; try (assumption). apply IHns. assumption.
+  Qed.
+
+  Lemma lookup_none : forall (n : N) (ns ns' : alist N V),
+      lookup n ns = None ->
+      lookup n (ns ++ ns') = lookup n ns'.
+  Proof.
+    intros n ns ns'.
+    generalize dependent ns'.
+    induction ns; intros ns'.
+    - reflexivity.
+    - destruct a.
+      assert ({n = n0} + {n <> n0}) as loem by apply (classicT (n = n0)).
+      destruct loem; simpl.
+      + rewrite e. rewrite 2 If_l; try (reflexivity). intro H. inversion H.
+      + rewrite 2 If_r; try (assumption). apply IHns.
+  Qed.
+
+  Lemma lookup_same : forall (n : N) (ns : alist N V),
+      lookup n (ns ++ ns) = lookup n ns.
+  Proof.
+    intros n ns.
+    destruct (lookup n ns) eqn:H; rewrite <- H.
+    - apply lookup_cover with v; assumption.
+    - apply lookup_none; assumption.
+  Qed.
+End LookupTheory.
+
+Section NamespaceTheory.
+  Variable M : Type.
+  Variable N : Type.
+  Variable V : Type.
+
+  Lemma get_modded_namespace_append : forall (ns ns' : namespace M N V) (x : M),
+      get_modded_namespace x (ns ++ ns') = (get_modded_namespace x ns) ++ (get_modded_namespace x ns').
+  Proof.
+    induction ns; intros ns' x.
+    - reflexivity.
+    - destruct a. destruct i.
+      + apply IHns.
+      + simpl. assert ({x = m} + {x <> m}) as loem by (apply (classicT (x = m))).
+        destruct loem.
+        * rewrite <- e. rewrite 2 If_l; try (reflexivity). unfold app. simpl. rewrite IHns. reflexivity.
+        * rewrite 2 If_r; try (assumption). apply IHns.
+  Qed.
+
+  Lemma nsLookup_empty : forall (id : ident M N), nsLookup id ([] : namespace M N V) = None.
+  Proof.
+    reflexivity.
+  Qed.
+
+  Lemma nsLookup_cover : forall (id : ident M N) (ns ns' : namespace M N V) (v : V),
+      nsLookup id ns = Some v ->
+      nsLookup id (ns ++ ns') = nsLookup id ns.
+  Proof.
+    intros. unfold nsLookup in *. apply lookup_cover with v. assumption.
+  Qed.
+
+  Lemma nsLookup_drop : forall (id : ident M N) (ns ns' : namespace M N V),
+      nsLookup id ns = None ->
+      nsLookup id (ns ++ ns') = nsLookup id ns'.
+  Proof.
+    intros id ns ns' H.
+    unfold nsLookup in *. apply lookup_drop. assumption.
+  Qed.
+
+  Lemma nsLookup_same : forall (id : ident M N) (ns : namespace M N V),
+      nsLookup id (ns ++ ns) = nsLookup id ns.
+  Proof.
+    intros id ns.
+    unfold nsLookup in *. apply lookup_same.
+  Qed.
+
+End NamespaceTheory.
